doc.lisp
@@ -33532,6 +33532,29 @@ INFORMAL INTRODUCTION
   known stobj.  In fact, stobjs are not allowed to be declared in
   [47mWITH[0m clauses (and that is not necessary for assigning to them).
 
+  Note that it is possible to write [47mDO[0m loops without any [47mWITH[0m clauses,
+  provided a stobj is being manipulated and measured in the body.
+  For example, using the stobj declared in the previous example,
+
+    (loop$ do
+           :values (st)
+           :measure (acl2-count (fld st))
+           (if (endp (fld st))
+               (return st)
+               (if (equal 3 (car (fld st)))
+                   (return st)
+                   (setq st (update-fld (cdr (fld st)) st)))))
+
+  is acceptable.  In Common Lisp, [47m(loop$ do <body>)[0m loops until a
+  [47mreturn[0m is executed and so to be admissible in ACL2 some [47m:measure[0m
+  must be specified (unless there is [47mreturn[0m on every branch through
+  [47m<body>[0m).  If there are no [47mWITH[0m clauses, stobjs are the only objects
+  that might be measured to explain termination, and ACL2 cannot
+  guess effective measures of stobjs.
+
+  To see some advice about proving inductive theorems about [47mDO[0m loops
+  measured by stobjs, see [stating-and-proving-lemmas-about-loop$s].
+
   [31;1mThe [47mOF-TYPE[0m[31;1m Keyword[0m
 
   So far our examples have all involved [47mloop$[0m expressions that are
@@ -67114,11 +67137,11 @@ Subtopics
     ***********************************************
 
   The solution is generally to [disable] the [executable-counterpart]
-  of the offending function.  As of this writing (in July, 2025), the
-  only way to get an unexpected ``live'' [stobj] is by the use of
-  [47m[swap-stobjs][0m, as suggested by the example shown below (essentially
-  provided by Sol Swords) --- which results in a different error
-  message, shown below, than the one above.
+  of the offending function.  It may well be that the only way to get
+  an unexpected ``live'' [stobj] is by the use of [47m[swap-stobjs][0m, as
+  suggested by the example shown below (essentially provided by Sol
+  Swords) --- which results in a different error message, shown
+  below, than the one above.
 
   First introduce a pair of congruent [stobj]s.
 
@@ -142957,6 +142980,104 @@ Normal Forms in [47mLoop$[0m Bodies
   [47mrev-loop$[0m is expanded.  Note that the [47mloop$[0m was written with [47m(endp
   tail)[0m in the [47mdefun[0m of [47mrev-loop$[0m but lemma deals with the normalized
   form of that body.
+
+  Here is another example, this one involving a [47mdo[0m loop without any
+  [47mWITH[0m clauses.  That in itself causes no special proof problems, but
+  as noted in [do-loop$], it necessitates the use of a stobj in the
+  body and that raises issues similar to those just mentioned.  So
+  below we introduce a stobj, [47mst[0m, with one field, [47mfld[0m.  We define
+  [47m[warrant][0ms for both [47mfld[0m and [47mupdate-fld[0m, and then we define a
+  function, [47mstobj-mem[0m, that uses a [47mdo[0m loop to determine whether a
+  given element occurs in the field, simultaneously shortening the
+  list in the field so that its [47mcar[0m is the element in question.  Here
+  is the setup.
+
+    (defstobj st fld)
+    (defwarrant fld)
+    (defwarrant update-fld)
+
+    (defun stobj-mem (e st)
+      (declare (xargs :stobjs (st)
+                      :guard (true-listp (fld st))))
+      (loop$ do
+             :values (st)
+             :guard (and (stp st)
+                         (true-listp (fld st)))
+             :measure (acl2-count (fld st))
+             (if (endp (fld st))
+                 (return st)
+                 (if (equal e (car (fld st)))
+                     (return st)
+                     (setq st (update-fld (cdr (fld st)) st))))))
+
+  Note that there is no [47mWITH[0m clause but the size of [47m(fld st)[0m is
+  decreasing.
+
+  Suppose we want to prove that after running [47m(stobj-mem e st)[0m on
+  proper input, the final value of [47mfld[0m is equal to [47m(member e (fld
+  st))[0m.  The desired formal statement is
+
+    (defthm stobj-mem-correct
+      (implies (and (stp st)
+                    (true-listp (fld st))
+                    (warrant fld update-fld))
+               (let ((st1 (stobj-mem e st)))
+                 (and (stp st1)
+                      (equal (fld st1)
+                             (member e (fld st))))))
+      :hints ...)
+
+  Note that in the theorem we use [47mst1[0m to denote the final value of the
+  stobj whose initial value is [47mst[0m.  We have to provide the warrants
+  for the accessor and updater used in the body of the [47mloop$[0m.
+
+  This theorem is a little tricky to prove because we're proving a
+  conjunction and after the [47m(stobj-mem e st)[0m and the [47m(stp st)[0m expand
+  we get several conjectures, each of which requires induction.  It
+  is simply easier to prove that the [47mloop$[0m in [47mstobj-mem[0m has the
+  desired property and then use that lemma.  So we first prove:
+
+    (defthm stobj-mem-correct-lemma
+      (implies (and (stp st)
+                    (true-listp (fld st))
+                    (warrant fld update-fld))
+               (let ((st1 (loop$ do
+                                 :values (st)
+                                 :guard (and (stp st)
+                                             (true-listp (fld st)))
+                                 :measure (acl2-count (fld st))
+                                 (if (consp (fld st))
+                                     (if (equal e (car (fld st)))
+                                         (return st)
+                                         (setq st (update-fld (cdr (fld st)) st)))
+                                     (return st)))))
+                 (and (stp st1)
+                      (equal (fld st1)
+                             (member e (fld st)))))))
+
+  But note that we expanded the [47mendp[0m in the statement of this lemma
+  because [47mendp[0m is built-in in a way that causes it often to expand
+  even when disabled (as is actually noted in a warning message if
+  we'd left the [47mendp[0m in place).  We also normalized the resulting [47m(if
+  (not (consp (fld st))) ...)[0m as explained in Lesson 2 above.
+
+  Now we'd like to prove the desired theorem about [47mstobj-mem[0m, expecting
+  that function to expand and then the lemma to hit it and complete
+  the proof.  But that won't work without a little more help!  The
+  problem is that the lemma mentions [47mstp[0m, [47mfld[0m, and [47mupdate-fld[0m in its
+  left-hand side and those are non-recursively defined functions that
+  will expand.  So to make the lemma match the rewritten main theorem
+  we must disable those three functions.
+
+    (defthm stobj-mem-correct
+      (implies (and (stp st)
+                    (true-listp (fld st))
+                    (warrant fld update-fld))
+               (let ((st1 (stobj-mem e st)))
+                 (and (stp st1)
+                      (equal (fld st1)
+                             (member e (fld st))))))
+      :hints ((\"Goal\" :in-theory (disable stp fld update-fld))))
 
 
 The Secret [47mSetq[0m Problem
